pcuic/theories/PCUICTyping.v
@@ -801,6 +801,8 @@ Module PCUICTypingDef <: Typing PCUICTerm PCUICEnvironment PCUICEnvTyping.
   Definition ind_guard := ind_guard.
   Definition typing := @typing.
   Definition smash_context := smash_context.
+  Definition lift_context := lift_context.
+  Definition subst_telescope := subst_telescope.
 
 End PCUICTypingDef.
 
@@ -1176,11 +1178,12 @@ Proof.
          simpl in IH. simpl. apply IH; constructor 1; simpl; lia.
       ++ pose proof Xg.(onConstructors) as Xg'.
          eapply All2_impl; eauto. intros.
-         red in X14 |- *. destruct X14 as [[s Hs] [cs Hargsu]]. split.
+         destruct X14 as [cs onctyp oncargs oncind].
+         unshelve econstructor. eauto.
+         destruct onctyp as [s Hs].
          pose proof (typing_wf_local (Σ:= (Σ, udecl)) Hs). simpl in Hs.
          specialize (IH (existT _ (Σ, udecl) (existT _ X13 (existT _ _ (existT _ X14 (existT _ _ (existT _ _ Hs))))))).
          simpl in IH. red. simpl. exists s. simpl. apply IH; constructor 1; simpl; auto with arith.
-         exists cs.
          eapply type_local_ctx_impl; eauto. simpl. intros. red in X14.
          destruct T.
          pose proof (typing_wf_local X14).
@@ -1189,6 +1192,13 @@ Proof.
          destruct X14 as [u Hu]. exists u.
          pose proof (typing_wf_local Hu).
          specialize (IH (existT _ (Σ, udecl) (existT _ X13 (existT _ _ (existT _ X14 (existT _ _ (existT _ _ Hu))))))).
+         apply IH. simpl. constructor 1. simpl. auto with arith.
+         clear -X13 IH oncind.
+         revert oncind.
+         generalize (List.rev (lift_context #|cshape_args cs| 0 (ind_indices Xg))).
+         generalize (cshape_indices cs). induction 1; constructor; auto.
+         red in p0 |- *.
+         specialize (IH (existT _ (Σ, udecl) (existT _ X13 (existT _ _ (existT _ (typing_wf_local p0) (existT _ _ (existT _ _ p0))))))).
          apply IH. simpl. constructor 1. simpl. auto with arith.
       ++ intros Hprojs; pose proof (onProjections Xg Hprojs); auto. simpl in *.
          destruct X14; constructor; auto. eapply Alli_impl; eauto. clear on_projs0. intros.
